An attribute `assume_strictly_positive` to selectively admit the positivity check (used on FStar.Monotonic.mref)

src/parser/FStar.Parser.Const.fs
@@ -256,6 +256,7 @@ let dm4f_bind_range_attr = p2l ["FStar"; "Pervasives"; "dm4f_bind_range"]
 let must_erase_for_extraction_attr = psconst "must_erase_for_extraction"
 let fail_attr      = psconst "fail"
 let fail_lax_attr  = psconst "fail_lax"
+let assume_strictly_positive_attr_lid = p2l ["FStar"; "Pervasives"; "assume_strictly_positive"]
 
 let gen_reset =
     let x = U.mk_ref 0 in
