ulib/FStar.Monotonic.Heap.fsti
@@ -18,6 +18,7 @@ val equal_extensional (h1:heap) (h2:heap)
 
 val emp :heap
 
+[@ assume_strictly_positive]
 val mref (a:Type0) (rel:preorder a) :Type0
 
 val addr_of: #a:Type0 -> #rel:preorder a -> mref a rel -> GTot nat
